convert SET_Protocol to use Nat_Bijection library

src/HOL/SET_Protocol/Message_SET.thy
@@ -7,7 +7,7 @@
 header{*The Message Theory, Modified for SET*}
 
 theory Message_SET
-imports Main Nat_Int_Bij
+imports Main Nat_Bijection
 begin
 
 subsection{*General Lemmas*}
@@ -81,17 +81,16 @@ translations
 
 
 definition nat_of_agent :: "agent => nat" where
-   "nat_of_agent == agent_case (curry nat2_to_nat 0)
-                               (curry nat2_to_nat 1)
-                               (curry nat2_to_nat 2)
-                               (curry nat2_to_nat 3)
-                               (nat2_to_nat (4,0))"
+   "nat_of_agent == agent_case (curry prod_encode 0)
+                               (curry prod_encode 1)
+                               (curry prod_encode 2)
+                               (curry prod_encode 3)
+                               (prod_encode (4,0))"
     --{*maps each agent to a unique natural number, for specifications*}
 
 text{*The function is indeed injective*}
 lemma inj_nat_of_agent: "inj nat_of_agent"
-by (simp add: nat_of_agent_def inj_on_def curry_def
-              nat2_to_nat_inj [THEN inj_eq]  split: agent.split) 
+by (simp add: nat_of_agent_def inj_on_def curry_def prod_encode_eq split: agent.split) 
 
 
 constdefs
